Versions/CompositeView_Refines_ThreeStateVersionedMap.i.dfy
@@ -22,9 +22,34 @@ module CompositeView_Refines_ThreeStateVersionedMap {
   
   import UI
 
-  function I(s: A.Variables) : C.Variables
-  requires A.Inv(s)
+  inductive predicate Reachable(s: A.Variables)
   {
+    A.Init(s) || (exists s0, u :: Reachable(s0) && A.Next(s0, s, u))
+  }
+
+  inductive lemma ReachableImpliesInv(s: A.Variables)
+  requires Reachable(s)
+  ensures A.Inv(s)
+  ensures B.Inv(Ref_A.I(s))
+  {
+    if A.Init(s) {
+      A.InitImpliesInv(s);
+      Ref_A.RefinesInit(s);
+      B.InitImpliesInv(Ref_A.I(s));
+    } else {
+      var s0, u :| Reachable(s0) && A.Next(s0, s, u);
+      ReachableImpliesInv(s0);
+      A.NextPreservesInv(s0, s, u);
+      Ref_A.RefinesNext(s0, s, u);
+      B.NextPreservesInv(Ref_A.I(s0), Ref_A.I(s), u);
+    }
+  }
+
+  function I(s: A.Variables) : C.Variables
+  requires Reachable(s)
+  {
+    ReachableImpliesInv(s);
+
     Ref_B.I(
       Ref_A.I(s)
     )
@@ -41,11 +66,12 @@ module CompositeView_Refines_ThreeStateVersionedMap {
   }
 
   lemma RefinesNext(s: A.Variables, s': A.Variables, uiop: UI.Op)
-    requires A.Inv(s)
+    requires Reachable(s)
     requires A.Next(s, s', uiop)
-    ensures A.Inv(s')
+    ensures Reachable(s')
     ensures C.Next(I(s), I(s'), uiop)
   {
+    ReachableImpliesInv(s);
     Ref_A.RefinesNext(s, s', uiop);
     Ref_B.RefinesNext(
       Ref_A.I(s),
